wip: mTM_to_single

theories/L/Complexity/Reductions/TMGenNP/mTM_to_singleTapeTM.v
@@ -16,33 +16,36 @@ From Undecidability.TM Require Single.EncodeTapes Single.StepTM CaseList.
 Module ContainsEncoding.
   Section containsEncoding.
     Local Unset Implicit Arguments.
-    
+
     Context {sig:Type} {n:nat} {X:Type}.
     Context (d:sig) (encode : X -> list sig).
     (*Hypothesis (nonEmpty : forall x, encode x <> []).*)
 
     Definition Rel : pRel sig bool 1 :=
       fun tin '(yout, tout) =>
-        inhabited
-          (reflect
-             (exists t__L (x:X) t__R,
+        match yout with
+          true => exists (x:X) t__L t__R,
                  let t__x := encode x in
                  tin[@Fin0] = midtape t__L (hd d t__x) (tl t__x++t__R)
-                 /\ tout[@Fin0] = midtape (rev (removelast t__x)++ t__L) (last t__x d) t__R)
-             yout).
-    
+                 /\ tout[@Fin0] = midtape (rev (removelast t__x)++ t__L) (last t__x d) t__R
+        | false => forall t__L (x:X) t__R,
+            let t__x := encode x in
+            tin[@Fin0] <> midtape t__L (hd d t__x) (tl t__x++t__R)
+        end.
+
+
   End containsEncoding.
 End ContainsEncoding.
 
 From Coq.ssr Require Import ssrfun.
 Module CheckEncodesTape.
   Section checkEncodesTape.
-    
-    Import EncodeTapes StateWhile CaseList Mono Multi MoveToSymbol Switch If Combinators Option.
+
+    Import EncodeTapes StateWhile CaseList Mono Multi MoveToSymbol Copy Switch If Combinators Option.
     Context (sig:finType) (n:nat).
 
     Compute encode_tape (midtape [3;2;1] 4 [5;6;7]).
-  (*encode_tape = 
+    (*encode_tape =
     fun (sig : Type) (t : tape sig) =>
       match t with
       | niltape _ => [NilBlank]
@@ -51,7 +54,7 @@ Module CheckEncodesTape.
       | midtape ls m rs => LeftBlank false :: map UnmarkedSymbol (rev ls) ++ MarkedSymbol m :: map UnmarkedSymbol rs ++ [RightBlank false]
       end*)
     Notation sig__M := (FinType(EqType(sigTape sig))).
-    
+
     Definition d__sig :sigTape sig := NilBlank.
     Definition Rel : pRel sig__M bool 1 := ContainsEncoding.Rel d__sig (encode_tape (sig:=sig)).
 
@@ -70,67 +73,173 @@ Module CheckEncodesTape.
       end.
 
     Let M2 x :pTM sig__M bool 1 := if negb (Option.apply (@isMarked sig) false x)
-                         then Return Nop false
-                         else
-                           MoveToSymbol (fun x => isMarked x || isLeftBorder x || isRightBorder x) id;;
-                                        Relabel ReadChar (Option.apply isRightBorder false).
+                                 then Return Nop false
+                                 else
+                                   MoveToSymbol (fun x => isMarked x || isLeftBorder x || isRightBorder x) id;;
+                                   Relabel ReadChar (Option.apply isRightBorder false).
 
-    Let M1 (x : option (sigTape sig)): pTM sig__M bool 1:=
-           match x with
-             Some NilBlank => Return Nop true
-           | Some (LeftBlank b) =>
-             (if b then Nop
-              else Move R;; 
-                        MoveToSymbol (fun x => isMarked x || isLeftBorder x || isRightBorder x) id
-             );;
-              Switch ReadChar M2
-                  
-           | _ => Return Nop false
-           end.
-    
-    Definition M : pTM sig__M bool 1  :=
+    Definition caseFirstSymbol : pTM sig__M (bool+bool) 1:=
       Switch
-        ReadChar M1.
+        ReadChar
+        (fun x =>
+           match x with
+             Some NilBlank => Return Nop (inl true)
+           | Some (LeftBlank b) => Return Nop (inr b)
+           | _ => Return Nop (inl false)
+           end).
+
+    Definition M : pTM sig__M bool 1:=
+      Switch caseFirstSymbol
+             (fun x =>
+                match x with
+                  inl b => Return Nop b
+                | inr b =>
+                  (if b then Nop
+                   else Move R);;
+                  MoveToSymbol (fun x => isMarked x || isLeftBorder x || isRightBorder x) id;;
+                  Switch ReadChar M2
+                end).
+
 
     (** Verification*)
-    
-    
+
+
     Local Arguments Vector.to_list {A n} (!v).
-    
+
     Local Arguments plus : simpl never.
     Local Arguments mult : simpl never.
+    Local Arguments caseFirstSymbol : simpl never.
+
+    Tactic Notation "destruct" "_" "in" constr(H):=
+      match type of H with
+      | context[match ?X with _ => _ end] => destruct X
+      | context[match ?X with _ => _ end] => destruct X
+      end.
+
+    Tactic Notation "tacInEvar" constr(E) tactic3(tac) :=
+      is_evar E;
+      let t := type of E in
+      let __tmp_callInEvar := fresh "__tmp_callInEvar" in
+      evar (__tmp_callInEvar:t);
+      (only [__tmp_callInEvar]:tac);unify E __tmp_callInEvar;subst __tmp_callInEvar;instantiate.
+
+    Tactic Notation "introsSwitch" ne_simple_intropattern_list(P):=
+      match goal with
+        |- (forall f' , _ ⊨ ?R f') =>
+        tacInEvar R intros P;cbn beta;intros P
+      end.
 
 
-    (*
+
+    Tactic Notation "destructBoth" constr(g) "as" simple_intropattern(P) :=
+      match goal with
+        |- (_ ⊨ ?R) =>
+        tacInEvar R (destruct g as P);destruct g as P;cbn zeta iota
+      end.
+
     Lemma Realises : M ⊨ Rel.
     Proof.
       eapply Realise_monotone.
-      { unfold M. TM_Correct.
-        all:unfold M1. all:TM_Correct.
-        all:unfold M2. all:cbn;TM_Correct.
+      { unfold M. apply Switch_Realise
+                    with (R1 :=
+                            fun tin '(yout, tout) =>
+                              tin = tout /\
+                              match yout with
+                                inl true => current tin[@Fin0] = Some NilBlank
+                              | inr b => current tin[@Fin0] = Some (LeftBlank b)
+                              | inl false => (forall b, current tin[@Fin0] <> Some (LeftBlank b)) /\ current tin[@Fin0] <> Some NilBlank
+                              end).
+        { eapply Realise_monotone.
+          {unfold caseFirstSymbol. TM_Correct. }
+          hnf;cbn. intros t0 [y1 t1]. intros (?&?&[-> ->]&H__cur).
+          repeat destruct _ in H__cur. all:revert H__cur;cbn. all:intros (->&_&->).
+          all:split;[easy| ]. all:intuition congruence.
+        }
+
+        introsSwitch [[]| b]. 1,2:now cbn;refine (Return_Realise _); TM_Correct.
+        eapply Seq_Realise. 1:now destructBoth b as []; TM_Correct.
+        TM_Correct_step. now TM_Correct.
+
+        apply Switch_Realise. now TM_Correct.
+        unfold M2;cbn. introsSwitch opt.
+        destructBoth (negb (oapp (isMarked (sig:=eqType_X (type sig))) false opt)) as []. TM_Correct. TM_Correct.
       }
-      { unfold Rel,ContainsEncoding.Rel. TMSimp. eauto. }
-      eapply TerminatesIn_monotone.
-      { unfold M. TM_Correct.
-        - apply Step_Realise.
-        - apply Step_Terminates. }
-      { revert q. apply StateWhileCoInduction; intros q; intros. destruct HT as (T&kn&outc&HLoop&HEncT&Hk). rewrite Loop_steps_eq in Hk. unfold Step_T, Step_Rel.
-        destruct (halt q) eqn:E; cbn in *.
-        - exists 0. split; auto. intros ymid tmid HStep. specialize HStep with (1 := HEncT) as (HStep&->). auto.
-        - destruct kn as [ | kn']; cbn in *.
-          + unfold haltConf in HLoop. cbn in HLoop. rewrite E in HLoop. congruence.
-          + unfold haltConf in HLoop. cbn in HLoop. rewrite E in HLoop.
-            destruct (trans (q, current_chars T)) as [q' acts] eqn:E2.
-            exists (Step_steps q T). repeat split. eauto.
-            intros ymid tmid HStep. specialize HStep with (1 := HEncT).
-            assert (step (mk_mconfig q T) = mk_mconfig q' (doAct_multi T acts)) as Hstep.
-            { unfold step. cbn. rewrite E2. reflexivity. }
-            rewrite Hstep in HStep. destruct HStep as (HStep&->).
-            exists (Loop_steps q' (doAct_multi T acts) kn'). repeat split; auto.
-            hnf. do 3 eexists. repeat split. 2: eauto. rewrite <- Hstep. eauto. eauto.
-      }
-    Qed.*)
-    
+      unfold Rel,ContainsEncoding.Rel. hnf;cbn.
+      intros t0 (l1&t1). intros (read1&?&(<-&?)&H');revert H'. destruct read1 as [[]| ];cbn.
+      -intros (->&_&->). destruct t0[@Fin0];inv H.
+       eexists (@niltape sig),_,_. repeat split.
+      -intros (->&_&->). intros ? [] ?;destruct t0[@Fin0];cbn in H|-*;easy.
+      -intros ([]&t2&Ht2&_&t3&Ht3&?&?&[-> ->]&H');revert H'.
+       (*destruct (current t3[@Fin0]) eqn:H__cur;cbn.
+       2:{intros (->&?&<-). destruct b;cbn in Ht2.
+          - subst t2. destruct t1[@Fin0];cbn in *;try easy. *)
+
+       Lemma MoveToSymbol_id_spec (f:sig -> bool) t t' :
+         MoveToSymbol_Fun f id t = t' <-> ((current t = None /\ t = t')
+                                        \/ (exists t__L c t__R1 t__R2,
+                                              t = midtape t__L c (t__R1++t__R2)
+                                              /\ (forall x, x el removelast (c::t__R1) -> f x = false)
+                                              /\ tape_local_l t' = (rev (c::t__R1)++t__L)
+                                              /\ right t' = t__R2)). 
+       Proof.
+         clear n M2.
+         remember (tape_local t) as A eqn:eqA.
+         revert t t' eqA.
+         induction A using (size_induction (f:=@length sig));intros t t' eqA.
+         rewrite MoveToSymbol_Fun_equation. destruct current eqn:eq.
+         2:{ split. now left. intros [ | H']. easy. destruct H' as (?&?&?&?&->&?). easy. }
+         destruct f eqn:Hf.
+         { destruct t;inv eq. all:cbn. split.
+           -intros <-. right. eexists _,_,[],_.
+            repeat split. now intros ? [].
+           -intros [ | (?&?&?&?&[= -> -> -> ]&Hann&H''&<-)];[ easy | ].
+            destruct t';cbn in H''|-*. all:autorewrite with list in *.
+            all:try solve [apply (f_equal (@length _)) in H'';repeat (cbn in H'';autorewrite with list in H'');nia].
+            destruct x1. 2:{ exfalso. erewrite Hann in Hf. all:easy. }  cbn in *. congruence.
+         }
+         destruct t. all:inv eq. destruct l0. all:cbn - [removelast].
+         all:rewrite H;[ | | reflexivity];[ | cbn;nia].
+         - Fail. cbn. 
+         -
+           all:cbn cbn [doAct]. 
+                               +destruct l0. 2:easy. ccbn. subst. congruence. 2:rewrite <- H0;cbn.  2:split. intuition. easy. split. 
+         split.
+         2:{ intros [[H <-] | H].
+             -rewrite MoveToSymbol_Step_Fun_M2_None. 2:easy. unfold MoveToSymbol_Step_Fun. now rewrite H.
+             -destruct H as (?&?&?&?&->&Hall&Hleft&Hright).
+              erewrite MoveToSymbol_correct.
+         (* MoveToSymbol_correct:
+  forall (sig : finType) (stop : eqType_X (type sig) -> bool) (f : eqType_X (type sig) -> eqType_X (type sig))
+    (t : tape (eqType_X (type sig))) (str1 str2 : list (eqType_X (type sig))) (x : eqType_X (type sig)),
+  (forall x0 : eqType_X (type sig), x0 el str1 -> stop x0 = false) ->
+  stop x = true ->
+  tape_local t = str1 ++ x :: str2 -> MoveToSymbol_Fun stop f t = midtape (rev (List.map f str1) ++ left t) (f x) str2 *)
+       destruct (current.
+
+       Fail.
+       repeat eexists.
+       { unfold Rel,ContainsEncoding.Rel. TMSimp. eauto. }
+       eapply TerminatesIn_monotone.
+       { unfold M. TM_Correct.
+         - apply Step_Realise.
+         - apply Step_Terminates. }
+       { revert q. apply StateWhileCoInduction; intros q; intros. destruct HT as (T&kn&outc&HLoop&HEncT&Hk). rewrite Loop_steps_eq in Hk. unfold Step_T, Step_Rel.
+         destruct (halt q) eqn:E; cbn in *.
+         - exists 0. split; auto. intros ymid tmid HStep. specialize HStep with (1 := HEncT) as (HStep&->). auto.
+         - destruct kn as [ | kn']; cbn in *.
+           + unfold haltConf in HLoop. cbn in HLoop. rewrite E in HLoop. congruence.
+           + unfold haltConf in HLoop. cbn in HLoop. rewrite E in HLoop.
+             destruct (trans (q, current_chars T)) as [q' acts] eqn:E2.
+             exists (Step_steps q T). repeat split. eauto.
+             intros ymid tmid HStep. specialize HStep with (1 := HEncT).
+             assert (step (mk_mconfig q T) = mk_mconfig q' (doAct_multi T acts)) as Hstep.
+             { unfold step. cbn. rewrite E2. reflexivity. }
+             rewrite Hstep in HStep. destruct HStep as (HStep&->).
+             exists (Loop_steps q' (doAct_multi T acts) kn'). repeat split; auto.
+             hnf. do 3 eexists. repeat split. 2: eauto. rewrite <- Hstep. eauto. eauto.
+       }
+    Qed.
+
     Definition Ter : tRel sig__M 1:=
       fun tin k => 10 + sizeOfTape tin[@Fin0]*cnst 1 <= k.
 
@@ -143,10 +252,10 @@ Module CheckEncodesTape.
       }
       { intros tin k Hk. evar (k0:nat). enough (k0=k) as Hk0. rewrite <- Hk0. unfold k0.
         Tactic Notation "infArgs" int_or_var(n) := do n (try first [eexists | reflexivity]).
-        cbn. infArgs 5.  intros ? ? [-> ->].
-        (*TODO: unify cases *)
+                                                      cbn. infArgs 5.  intros ? ? [-> ->].
+                                                      (*TODO: unify cases *)
     Abort.
-    
+
   End checkEncodesTape.
 End CheckEncodesTape.
 
@@ -157,26 +266,26 @@ Module CheckEncodesTapes.
     Context (sig:finType) (n:nat).
 
     Eval cbv in encode_tapes [| niltape nat; midtape [3;2;1] 4 [5;6;7]; leftof 1 [2;3];rightof 3 [2;1] |].
-    
+
     Definition M__Rel : pRel sig 1
 
     Definition state := option (Fin.t n).
-    
-    
+
+
     Definition Step : pTM sig (state + bool) 1 := _.
-    
-    Definition M := StateWhile Step__CheckEncodeTapes. 
+
+    Definition M := StateWhile Step__CheckEncodeTapes.
     End checkEncodeTapes.
  *)
 
 Section multiToMono.
-  
+
   Import EncodeTapes.
   Context (sig F:finType) (n:nat) `{R__sig : registered sig}  (M : pTM sig F (S n)).
 
   Eval cbn in (StepTM.ToSingleTape M).
 
-  
+
 
 End multiToMono.
 
@@ -185,5 +294,5 @@ Lemma LMGenNP_to_TMGenNP_mTM (sig:finType) (n:nat) `{R__sig : registered sig}  (
     restrictBy (HaltsOrDiverges_fixed_mTM M) (TMGenNP_fixed_mTM M)
                ⪯p unrestrictedP (TMGenNP_fixed_singleTapeTM M').
 Proof.
-  
+
 Abort.
